DenotSem/Denot.thy
@@ -7,11 +7,12 @@ abbreviation fun_app :: "ty \<Rightarrow> ty \<Rightarrow> ty set" (infix "\<bul
 
 abbreviation up :: "ty \<Rightarrow> ty set" ("\<up>" 1000) where
   "up A \<equiv> {B. A <: B \<and> wf_ty B}"
-  
+
 fun E :: "exp \<Rightarrow> ty list \<Rightarrow> ty set" ("\<lbrakk>_\<rbrakk>_" [999] 1000) where
   Enat: "\<lbrakk>ENat n\<rbrakk> \<rho> = { TNat n }" |
   Evar: "\<lbrakk>EVar k\<rbrakk> \<rho> = (if k < length \<rho> then \<up>(\<rho>!k) else {})" |
-  Elam: "\<lbrakk>ELam e\<rbrakk> \<rho> = { f. wf_ty f \<and> (\<forall>v v'. v\<rightarrow>v' \<in> atoms f \<longrightarrow> v' \<in> \<lbrakk>e\<rbrakk>(v#\<rho>)) }" |
+  Elam: "\<lbrakk>ELam e\<rbrakk> \<rho> = { f. wf_ty f \<and> all_funs (atoms f) 
+                          \<and> (\<forall>v v'. v\<rightarrow>v' \<in> atoms f \<longrightarrow> v' \<in> \<lbrakk>e\<rbrakk>(v#\<rho>)) }" |
   Eapp: "\<lbrakk>EApp e1 e2\<rbrakk> \<rho> = { v'. \<exists> f v. f \<in> \<lbrakk>e1\<rbrakk>\<rho> \<and> v \<in> \<lbrakk>e2\<rbrakk>\<rho> \<and> v' \<in> f \<bullet> v }" | 
   Eprim: "\<lbrakk>EPrim f e1 e2\<rbrakk> \<rho> = { v. \<exists> v1 v2 n1 n2. v1 \<in> \<lbrakk>e1\<rbrakk>\<rho> 
           \<and> v2 \<in> \<lbrakk>e2\<rbrakk>\<rho> \<and> v1 \<approx> TNat n1 \<and> v2 \<approx> TNat n2 \<and> v \<approx> TNat (f n1 n2) }" |
